Test/Passes/InstructionSelection/RISCV64/fastntt.mlir
@@ -1,4 +1,4 @@
-// RUN: veir-opt %s -p=isel-br-riscv64,isel-riscv64,reconcile-cast,riscv-combine | filecheck %s
+// RUN: veir-opt %s -p=isel-sdag-riscv64,isel-br-riscv64,isel-riscv64,reconcile-cast,riscv-combine,dce | filecheck %s
 
 "builtin.module"() ({
   ^4():
@@ -118,146 +118,160 @@
 // CHECK-NEXT:     "llvm.module_flags"() {{.*}} : () -> ()
 // CHECK-NEXT:     "llvm.func"() <{{{.*}}"sym_name" = "fastNTT"{{.*}}}> ({
 // CHECK-NEXT:       ^[[bb7:[0-9]+]](%[[varg7_0:[a-zA-Z0-9_]+]] : !llvm.ptr, %[[varg7_1:[a-zA-Z0-9_]+]] : i64, %[[varg7_2:[a-zA-Z0-9_]+]] : i64, %[[varg7_3:[a-zA-Z0-9_]+]] : !llvm.ptr, %[[varg7_4:[a-zA-Z0-9_]+]] : i64, %[[varg7_5:[a-zA-Z0-9_]+]] : i64):
-// CHECK-NEXT:         %[[v374:[0-9]+]] = "rv64.get_register"() : () -> !riscv.reg<x0>
-// CHECK-NEXT:         %[[v370:[0-9]+]] = "riscv.li"() <{"value" = 2 : i64}> : () -> !riscv.reg
-// CHECK-NEXT:         %[[v368:[0-9]+]] = "riscv.li"() <{"value" = 1 : i64}> : () -> !riscv.reg
-// CHECK-NEXT:         %[[v363:[0-9]+]] = "builtin.unrealized_conversion_cast"(%[[varg7_4]]) : (i64) -> !riscv.reg
-// CHECK-NEXT:         %[[v375:[0-9]+]] = "rv64.get_register"() : () -> !riscv.reg<x0>
-// CHECK-NEXT:         %[[v366:[0-9]+]] = "riscv.sltu"(%[[v375]], %[[v363]]) : (!riscv.reg<x0>, !riscv.reg) -> !riscv.reg
-// CHECK-NEXT:         %[[v367:[0-9]+]] = "builtin.unrealized_conversion_cast"(%[[v366]]) : (!riscv.reg) -> i1
-// CHECK-NEXT:         %[[v114:[0-9]+]] = "builtin.unrealized_conversion_cast"(%[[v367]]) : (i1) -> !riscv.reg
-// CHECK-NEXT:         "riscv_cf.bnez"(%[[v114]]) [^[[bb12:[0-9]+]], ^[[bb13:[0-9]+]]] <{"operandSegmentSizes" = array<i32: 1, 0, 0>}> : (!riscv.reg) -> ()
+// CHECK-NEXT:         %[[v382:[0-9]+]] = "rv64.get_register"() : () -> !riscv.reg<x0>
+// CHECK-NEXT:         %[[v378:[0-9]+]] = "riscv.li"() <{"value" = 2 : i64}> : () -> !riscv.reg
+// CHECK-NEXT:         %[[v376:[0-9]+]] = "riscv.li"() <{"value" = 1 : i64}> : () -> !riscv.reg
+// CHECK-NEXT:         %[[v371:[0-9]+]] = "builtin.unrealized_conversion_cast"(%[[varg7_4]]) : (i64) -> !riscv.reg
+// CHECK-NEXT:         %[[v383:[0-9]+]] = "rv64.get_register"() : () -> !riscv.reg<x0>
+// CHECK-NEXT:         %[[v374:[0-9]+]] = "riscv.sltu"(%[[v383]], %[[v371]]) : (!riscv.reg<x0>, !riscv.reg) -> !riscv.reg
+// CHECK-NEXT:         %[[v375:[0-9]+]] = "builtin.unrealized_conversion_cast"(%[[v374]]) : (!riscv.reg) -> i1
+// CHECK-NEXT:         %[[v174:[0-9]+]] = "builtin.unrealized_conversion_cast"(%[[v375]]) : (i1) -> !riscv.reg
+// CHECK-NEXT:         "riscv_cf.bnez"(%[[v174]]) [^[[bb12:[0-9]+]], ^[[bb13:[0-9]+]]] <{"operandSegmentSizes" = array<i32: 1, 0, 0>}> : (!riscv.reg) -> ()
 // CHECK-NEXT:       ^[[bb12]]():
-// CHECK-NEXT:         %[[v118:[0-9]+]] = "builtin.unrealized_conversion_cast"(%[[varg7_1]]) : (i64) -> !riscv.reg
-// CHECK-NEXT:         "riscv_cf.branch"(%[[v118]]) [^[[bb15:[0-9]+]]] : (!riscv.reg) -> ()
+// CHECK-NEXT:         %[[v178:[0-9]+]] = "builtin.unrealized_conversion_cast"(%[[varg7_1]]) : (i64) -> !riscv.reg
+// CHECK-NEXT:         "riscv_cf.branch"(%[[v178]]) [^[[bb15:[0-9]+]]] : (!riscv.reg) -> ()
 // CHECK-NEXT:       ^[[bb13]]():
-// CHECK-NEXT:         "riscv_cf.branch"(%[[v370]]) [^[[bb15]]] : (!riscv.reg) -> ()
+// CHECK-NEXT:         "riscv_cf.branch"(%[[v378]]) [^[[bb15]]] : (!riscv.reg) -> ()
 // CHECK-NEXT:       ^[[bb15]](%[[varg15_0:[a-zA-Z0-9_]+]] : !riscv.reg):
-// CHECK-NEXT:         %[[v358:[0-9]+]] = "builtin.unrealized_conversion_cast"(%[[varg7_4]]) : (i64) -> !riscv.reg
-// CHECK-NEXT:         %[[v376:[0-9]+]] = "rv64.get_register"() : () -> !riscv.reg<x0>
-// CHECK-NEXT:         %[[v361:[0-9]+]] = "riscv.sltu"(%[[v376]], %[[v358]]) : (!riscv.reg<x0>, !riscv.reg) -> !riscv.reg
-// CHECK-NEXT:         %[[v362:[0-9]+]] = "builtin.unrealized_conversion_cast"(%[[v361]]) : (!riscv.reg) -> i1
-// CHECK-NEXT:         %[[v122:[0-9]+]] = "builtin.unrealized_conversion_cast"(%[[v362]]) : (i1) -> !riscv.reg
-// CHECK-NEXT:         "riscv_cf.bnez"(%[[v122]]) [^[[bb19:[0-9]+]], ^[[bb20:[0-9]+]]] <{"operandSegmentSizes" = array<i32: 1, 0, 0>}> : (!riscv.reg) -> ()
+// CHECK-NEXT:         %[[v366:[0-9]+]] = "builtin.unrealized_conversion_cast"(%[[varg7_4]]) : (i64) -> !riscv.reg
+// CHECK-NEXT:         %[[v384:[0-9]+]] = "rv64.get_register"() : () -> !riscv.reg<x0>
+// CHECK-NEXT:         %[[v369:[0-9]+]] = "riscv.sltu"(%[[v384]], %[[v366]]) : (!riscv.reg<x0>, !riscv.reg) -> !riscv.reg
+// CHECK-NEXT:         %[[v370:[0-9]+]] = "builtin.unrealized_conversion_cast"(%[[v369]]) : (!riscv.reg) -> i1
+// CHECK-NEXT:         %[[v182:[0-9]+]] = "builtin.unrealized_conversion_cast"(%[[v370]]) : (i1) -> !riscv.reg
+// CHECK-NEXT:         "riscv_cf.bnez"(%[[v182]]) [^[[bb19:[0-9]+]], ^[[bb20:[0-9]+]]] <{"operandSegmentSizes" = array<i32: 1, 0, 0>}> : (!riscv.reg) -> ()
 // CHECK-NEXT:       ^[[bb19]]():
-// CHECK-NEXT:         "riscv_cf.branch"(%[[v368]]) [^[[bb22:[0-9]+]]] : (!riscv.reg) -> ()
+// CHECK-NEXT:         "riscv_cf.branch"(%[[v376]]) [^[[bb22:[0-9]+]]] : (!riscv.reg) -> ()
 // CHECK-NEXT:       ^[[bb20]]():
-// CHECK-NEXT:         %[[v354:[0-9]+]] = "builtin.unrealized_conversion_cast"(%[[varg7_5]]) : (i64) -> !riscv.reg
-// CHECK-NEXT:         %[[v356:[0-9]+]] = "riscv.div"(%[[v354]], %[[v370]]) : (!riscv.reg, !riscv.reg) -> !riscv.reg
-// CHECK-NEXT:         "riscv_cf.branch"(%[[v356]]) [^[[bb22]]] : (!riscv.reg) -> ()
+// CHECK-NEXT:         %[[v168:[0-9]+]] = "builtin.unrealized_conversion_cast"(%[[varg7_5]]) : (i64) -> !riscv.reg
+// CHECK-NEXT:         %[[v387:[0-9]+]] = "riscv.srli"(%[[v168]]) <{"value" = 63 : i64}> : (!riscv.reg) -> !riscv.reg
+// CHECK-NEXT:         %[[v171:[0-9]+]] = "riscv.add"(%[[v168]], %[[v387]]) : (!riscv.reg, !riscv.reg) -> !riscv.reg
+// CHECK-NEXT:         %[[v172:[0-9]+]] = "riscv.srai"(%[[v171]]) <{"value" = 1 : i64}> : (!riscv.reg) -> !riscv.reg
+// CHECK-NEXT:         "riscv_cf.branch"(%[[v172]]) [^[[bb22]]] : (!riscv.reg) -> ()
 // CHECK-NEXT:       ^[[bb22]](%[[varg22_0:[a-zA-Z0-9_]+]] : !riscv.reg):
-// CHECK-NEXT:         %[[v350:[0-9]+]] = "builtin.unrealized_conversion_cast"(%[[varg7_1]]) : (i64) -> !riscv.reg
-// CHECK-NEXT:         %[[v352:[0-9]+]] = "riscv.div"(%[[v350]], %[[v370]]) : (!riscv.reg, !riscv.reg) -> !riscv.reg
-// CHECK-NEXT:         "riscv_cf.branch"(%[[varg22_0]], %[[v352]], %[[v374]], %[[varg15_0]]) [^[[bb27:[0-9]+]]] : (!riscv.reg, !riscv.reg, !riscv.reg<x0>, !riscv.reg) -> ()
+// CHECK-NEXT:         %[[v162:[0-9]+]] = "builtin.unrealized_conversion_cast"(%[[varg7_1]]) : (i64) -> !riscv.reg
+// CHECK-NEXT:         %[[v388:[0-9]+]] = "riscv.srli"(%[[v162]]) <{"value" = 63 : i64}> : (!riscv.reg) -> !riscv.reg
+// CHECK-NEXT:         %[[v165:[0-9]+]] = "riscv.add"(%[[v162]], %[[v388]]) : (!riscv.reg, !riscv.reg) -> !riscv.reg
+// CHECK-NEXT:         %[[v166:[0-9]+]] = "riscv.srai"(%[[v165]]) <{"value" = 1 : i64}> : (!riscv.reg) -> !riscv.reg
+// CHECK-NEXT:         "riscv_cf.branch"(%[[varg22_0]], %[[v166]], %[[v382]], %[[varg15_0]]) [^[[bb27:[0-9]+]]] : (!riscv.reg, !riscv.reg, !riscv.reg<x0>, !riscv.reg) -> ()
 // CHECK-NEXT:       ^[[bb27]](%[[varg27_0:[a-zA-Z0-9_]+]] : !riscv.reg, %[[varg27_1:[a-zA-Z0-9_]+]] : !riscv.reg, %[[varg27_2:[a-zA-Z0-9_]+]] : !riscv.reg, %[[varg27_3:[a-zA-Z0-9_]+]] : !riscv.reg):
-// CHECK-NEXT:         %[[v150:[0-9]+]] = "builtin.unrealized_conversion_cast"(%[[varg7_1]]) : (i64) -> !riscv.reg
-// CHECK-NEXT:         "riscv_cf.branch"(%[[v374]], %[[v150]]) [^[[bb29:[0-9]+]]] : (!riscv.reg<x0>, !riscv.reg) -> ()
+// CHECK-NEXT:         %[[v210:[0-9]+]] = "builtin.unrealized_conversion_cast"(%[[varg7_1]]) : (i64) -> !riscv.reg
+// CHECK-NEXT:         "riscv_cf.branch"(%[[v382]], %[[v210]]) [^[[bb29:[0-9]+]]] : (!riscv.reg<x0>, !riscv.reg) -> ()
 // CHECK-NEXT:       ^[[bb29]](%[[varg29_0:[a-zA-Z0-9_]+]] : !riscv.reg, %[[varg29_1:[a-zA-Z0-9_]+]] : !riscv.reg):
-// CHECK-NEXT:         %[[v348:[0-9]+]] = "riscv.slt"(%[[v368]], %[[varg29_1]]) : (!riscv.reg, !riscv.reg) -> !riscv.reg
-// CHECK-NEXT:         %[[v349:[0-9]+]] = "builtin.unrealized_conversion_cast"(%[[v348]]) : (!riscv.reg) -> i1
-// CHECK-NEXT:         %[[v159:[0-9]+]] = "builtin.unrealized_conversion_cast"(%[[v349]]) : (i1) -> !riscv.reg
-// CHECK-NEXT:         "riscv_cf.bnez"(%[[v159]]) [^[[bb32:[0-9]+]], ^[[bb33:[0-9]+]]] <{"operandSegmentSizes" = array<i32: 1, 0, 0>}> : (!riscv.reg) -> ()
+// CHECK-NEXT:         %[[v364:[0-9]+]] = "riscv.slt"(%[[v376]], %[[varg29_1]]) : (!riscv.reg, !riscv.reg) -> !riscv.reg
+// CHECK-NEXT:         %[[v365:[0-9]+]] = "builtin.unrealized_conversion_cast"(%[[v364]]) : (!riscv.reg) -> i1
+// CHECK-NEXT:         %[[v219:[0-9]+]] = "builtin.unrealized_conversion_cast"(%[[v365]]) : (i1) -> !riscv.reg
+// CHECK-NEXT:         "riscv_cf.bnez"(%[[v219]]) [^[[bb32:[0-9]+]], ^[[bb33:[0-9]+]]] <{"operandSegmentSizes" = array<i32: 1, 0, 0>}> : (!riscv.reg) -> ()
 // CHECK-NEXT:       ^[[bb32]]():
-// CHECK-NEXT:         %[[v344:[0-9]+]] = "riscv.sra"(%[[varg29_1]], %[[v368]]) : (!riscv.reg, !riscv.reg) -> !riscv.reg
-// CHECK-NEXT:         %[[v340:[0-9]+]] = "riscv.add"(%[[v368]], %[[varg29_0]]) : (!riscv.reg, !riscv.reg) -> !riscv.reg
-// CHECK-NEXT:         "riscv_cf.branch"(%[[v340]], %[[v344]]) [^[[bb29]]] : (!riscv.reg, !riscv.reg) -> ()
+// CHECK-NEXT:         %[[v160:[0-9]+]] = "riscv.srai"(%[[varg29_1]]) <{"value" = 1 : i64}> : (!riscv.reg) -> !riscv.reg
+// CHECK-NEXT:         %[[v157:[0-9]+]] = "riscv.addi"(%[[varg29_0]]) <{"value" = 1 : i64}> : (!riscv.reg) -> !riscv.reg
+// CHECK-NEXT:         "riscv_cf.branch"(%[[v157]], %[[v160]]) [^[[bb29]]] : (!riscv.reg, !riscv.reg) -> ()
 // CHECK-NEXT:       ^[[bb33]]():
-// CHECK-NEXT:         %[[v336:[0-9]+]] = "riscv.slt"(%[[varg27_2]], %[[varg29_0]]) : (!riscv.reg, !riscv.reg) -> !riscv.reg
-// CHECK-NEXT:         %[[v337:[0-9]+]] = "builtin.unrealized_conversion_cast"(%[[v336]]) : (!riscv.reg) -> i1
-// CHECK-NEXT:         %[[v168:[0-9]+]] = "builtin.unrealized_conversion_cast"(%[[v337]]) : (i1) -> !riscv.reg
-// CHECK-NEXT:         "riscv_cf.bnez"(%[[v168]]) [^[[bb39:[0-9]+]], ^[[bb40:[0-9]+]]] <{"operandSegmentSizes" = array<i32: 1, 0, 0>}> : (!riscv.reg) -> ()
+// CHECK-NEXT:         %[[v360:[0-9]+]] = "riscv.slt"(%[[varg27_2]], %[[varg29_0]]) : (!riscv.reg, !riscv.reg) -> !riscv.reg
+// CHECK-NEXT:         %[[v361:[0-9]+]] = "builtin.unrealized_conversion_cast"(%[[v360]]) : (!riscv.reg) -> i1
+// CHECK-NEXT:         %[[v228:[0-9]+]] = "builtin.unrealized_conversion_cast"(%[[v361]]) : (i1) -> !riscv.reg
+// CHECK-NEXT:         "riscv_cf.bnez"(%[[v228]]) [^[[bb39:[0-9]+]], ^[[bb40:[0-9]+]]] <{"operandSegmentSizes" = array<i32: 1, 0, 0>}> : (!riscv.reg) -> ()
 // CHECK-NEXT:       ^[[bb39]]():
-// CHECK-NEXT:         "riscv_cf.branch"(%[[v374]]) [^[[bb42:[0-9]+]]] : (!riscv.reg<x0>) -> ()
+// CHECK-NEXT:         "riscv_cf.branch"(%[[v382]]) [^[[bb42:[0-9]+]]] : (!riscv.reg<x0>) -> ()
 // CHECK-NEXT:       ^[[bb42]](%[[varg42_0:[a-zA-Z0-9_]+]] : !riscv.reg):
-// CHECK-NEXT:         %[[v330:[0-9]+]] = "builtin.unrealized_conversion_cast"(%[[varg7_1]]) : (i64) -> !riscv.reg
-// CHECK-NEXT:         %[[v332:[0-9]+]] = "riscv.div"(%[[v330]], %[[varg27_3]]) : (!riscv.reg, !riscv.reg) -> !riscv.reg
-// CHECK-NEXT:         %[[v328:[0-9]+]] = "riscv.slt"(%[[varg42_0]], %[[v332]]) : (!riscv.reg, !riscv.reg) -> !riscv.reg
-// CHECK-NEXT:         %[[v329:[0-9]+]] = "builtin.unrealized_conversion_cast"(%[[v328]]) : (!riscv.reg) -> i1
-// CHECK-NEXT:         %[[v176:[0-9]+]] = "builtin.unrealized_conversion_cast"(%[[v329]]) : (i1) -> !riscv.reg
-// CHECK-NEXT:         "riscv_cf.bnez"(%[[v176]]) [^[[bb46:[0-9]+]], ^[[bb47:[0-9]+]]] <{"operandSegmentSizes" = array<i32: 1, 0, 0>}> : (!riscv.reg) -> ()
+// CHECK-NEXT:         %[[v354:[0-9]+]] = "builtin.unrealized_conversion_cast"(%[[varg7_1]]) : (i64) -> !riscv.reg
+// CHECK-NEXT:         %[[v356:[0-9]+]] = "riscv.div"(%[[v354]], %[[varg27_3]]) : (!riscv.reg, !riscv.reg) -> !riscv.reg
+// CHECK-NEXT:         %[[v352:[0-9]+]] = "riscv.slt"(%[[varg42_0]], %[[v356]]) : (!riscv.reg, !riscv.reg) -> !riscv.reg
+// CHECK-NEXT:         %[[v353:[0-9]+]] = "builtin.unrealized_conversion_cast"(%[[v352]]) : (!riscv.reg) -> i1
+// CHECK-NEXT:         %[[v236:[0-9]+]] = "builtin.unrealized_conversion_cast"(%[[v353]]) : (i1) -> !riscv.reg
+// CHECK-NEXT:         "riscv_cf.bnez"(%[[v236]]) [^[[bb46:[0-9]+]], ^[[bb47:[0-9]+]]] <{"operandSegmentSizes" = array<i32: 1, 0, 0>}> : (!riscv.reg) -> ()
 // CHECK-NEXT:       ^[[bb46]]():
-// CHECK-NEXT:         "riscv_cf.branch"(%[[v374]]) [^[[bb49:[0-9]+]]] : (!riscv.reg<x0>) -> ()
+// CHECK-NEXT:         "riscv_cf.branch"(%[[v382]]) [^[[bb49:[0-9]+]]] : (!riscv.reg<x0>) -> ()
 // CHECK-NEXT:       ^[[bb49]](%[[varg49_0:[a-zA-Z0-9_]+]] : !riscv.reg):
-// CHECK-NEXT:         %[[v324:[0-9]+]] = "riscv.div"(%[[varg27_3]], %[[v370]]) : (!riscv.reg, !riscv.reg) -> !riscv.reg
-// CHECK-NEXT:         %[[v320:[0-9]+]] = "riscv.slt"(%[[varg49_0]], %[[v324]]) : (!riscv.reg, !riscv.reg) -> !riscv.reg
-// CHECK-NEXT:         %[[v321:[0-9]+]] = "builtin.unrealized_conversion_cast"(%[[v320]]) : (!riscv.reg) -> i1
-// CHECK-NEXT:         %[[v183:[0-9]+]] = "builtin.unrealized_conversion_cast"(%[[v321]]) : (i1) -> !riscv.reg
-// CHECK-NEXT:         "riscv_cf.bnez"(%[[v183]]) [^[[bb53:[0-9]+]], ^[[bb54:[0-9]+]]] <{"operandSegmentSizes" = array<i32: 1, 0, 0>}> : (!riscv.reg) -> ()
+// CHECK-NEXT:         %[[v389:[0-9]+]] = "riscv.srli"(%[[varg27_3]]) <{"value" = 63 : i64}> : (!riscv.reg) -> !riscv.reg
+// CHECK-NEXT:         %[[v153:[0-9]+]] = "riscv.add"(%[[varg27_3]], %[[v389]]) : (!riscv.reg, !riscv.reg) -> !riscv.reg
+// CHECK-NEXT:         %[[v154:[0-9]+]] = "riscv.srai"(%[[v153]]) <{"value" = 1 : i64}> : (!riscv.reg) -> !riscv.reg
+// CHECK-NEXT:         %[[v348:[0-9]+]] = "riscv.slt"(%[[varg49_0]], %[[v154]]) : (!riscv.reg, !riscv.reg) -> !riscv.reg
+// CHECK-NEXT:         %[[v349:[0-9]+]] = "builtin.unrealized_conversion_cast"(%[[v348]]) : (!riscv.reg) -> i1
+// CHECK-NEXT:         %[[v243:[0-9]+]] = "builtin.unrealized_conversion_cast"(%[[v349]]) : (i1) -> !riscv.reg
+// CHECK-NEXT:         "riscv_cf.bnez"(%[[v243]]) [^[[bb53:[0-9]+]], ^[[bb54:[0-9]+]]] <{"operandSegmentSizes" = array<i32: 1, 0, 0>}> : (!riscv.reg) -> ()
 // CHECK-NEXT:       ^[[bb53]]():
-// CHECK-NEXT:         %[[v316:[0-9]+]] = "riscv.mul"(%[[varg27_3]], %[[varg42_0]]) : (!riscv.reg, !riscv.reg) -> !riscv.reg
-// CHECK-NEXT:         %[[v312:[0-9]+]] = "riscv.add"(%[[varg49_0]], %[[v316]]) : (!riscv.reg, !riscv.reg) -> !riscv.reg
-// CHECK-NEXT:         %[[v306:[0-9]+]] = "builtin.unrealized_conversion_cast"(%[[varg7_0]]) : (!llvm.ptr) -> !riscv.reg
-// CHECK-NEXT:         %[[v308:[0-9]+]] = "riscv.sh3add"(%[[v312]], %[[v306]]) : (!riscv.reg, !riscv.reg) -> !riscv.reg
-// CHECK-NEXT:         %[[v304:[0-9]+]] = "riscv.ld"(%[[v308]]) <{"value" = 0 : i64}> : (!riscv.reg) -> !riscv.reg
-// CHECK-NEXT:         %[[v301:[0-9]+]] = "riscv.div"(%[[varg27_3]], %[[v370]]) : (!riscv.reg, !riscv.reg) -> !riscv.reg
-// CHECK-NEXT:         %[[v297:[0-9]+]] = "riscv.add"(%[[v301]], %[[v312]]) : (!riscv.reg, !riscv.reg) -> !riscv.reg
-// CHECK-NEXT:         %[[v291:[0-9]+]] = "builtin.unrealized_conversion_cast"(%[[varg7_0]]) : (!llvm.ptr) -> !riscv.reg
-// CHECK-NEXT:         %[[v293:[0-9]+]] = "riscv.sh3add"(%[[v297]], %[[v291]]) : (!riscv.reg, !riscv.reg) -> !riscv.reg
-// CHECK-NEXT:         %[[v289:[0-9]+]] = "riscv.ld"(%[[v293]]) <{"value" = 0 : i64}> : (!riscv.reg) -> !riscv.reg
-// CHECK-NEXT:         %[[v286:[0-9]+]] = "riscv.mul"(%[[varg49_0]], %[[v370]]) : (!riscv.reg, !riscv.reg) -> !riscv.reg
-// CHECK-NEXT:         %[[v282:[0-9]+]] = "riscv.add"(%[[v368]], %[[v286]]) : (!riscv.reg, !riscv.reg) -> !riscv.reg
-// CHECK-NEXT:         %[[v278:[0-9]+]] = "riscv.mul"(%[[varg27_1]], %[[v282]]) : (!riscv.reg, !riscv.reg) -> !riscv.reg
-// CHECK-NEXT:         %[[v272:[0-9]+]] = "builtin.unrealized_conversion_cast"(%[[varg7_3]]) : (!llvm.ptr) -> !riscv.reg
-// CHECK-NEXT:         %[[v274:[0-9]+]] = "riscv.sh3add"(%[[v278]], %[[v272]]) : (!riscv.reg, !riscv.reg) -> !riscv.reg
-// CHECK-NEXT:         %[[v270:[0-9]+]] = "riscv.ld"(%[[v274]]) <{"value" = 0 : i64}> : (!riscv.reg) -> !riscv.reg
-// CHECK-NEXT:         %[[v267:[0-9]+]] = "riscv.mul"(%[[v289]], %[[v270]]) : (!riscv.reg, !riscv.reg) -> !riscv.reg
-// CHECK-NEXT:         %[[v262:[0-9]+]] = "builtin.unrealized_conversion_cast"(%[[varg7_2]]) : (i64) -> !riscv.reg
-// CHECK-NEXT:         %[[v263:[0-9]+]] = "riscv.rem"(%[[v267]], %[[v262]]) : (!riscv.reg, !riscv.reg) -> !riscv.reg
-// CHECK-NEXT:         %[[v259:[0-9]+]] = "riscv.add"(%[[v263]], %[[v304]]) : (!riscv.reg, !riscv.reg) -> !riscv.reg
-// CHECK-NEXT:         %[[v254:[0-9]+]] = "builtin.unrealized_conversion_cast"(%[[varg7_2]]) : (i64) -> !riscv.reg
-// CHECK-NEXT:         %[[v255:[0-9]+]] = "riscv.rem"(%[[v259]], %[[v254]]) : (!riscv.reg, !riscv.reg) -> !riscv.reg
-// CHECK-NEXT:         %[[v251:[0-9]+]] = "riscv.sub"(%[[v304]], %[[v263]]) : (!riscv.reg, !riscv.reg) -> !riscv.reg
-// CHECK-NEXT:         %[[v246:[0-9]+]] = "builtin.unrealized_conversion_cast"(%[[varg7_2]]) : (i64) -> !riscv.reg
-// CHECK-NEXT:         %[[v247:[0-9]+]] = "riscv.add"(%[[v246]], %[[v251]]) : (!riscv.reg, !riscv.reg) -> !riscv.reg
-// CHECK-NEXT:         %[[v242:[0-9]+]] = "builtin.unrealized_conversion_cast"(%[[varg7_2]]) : (i64) -> !riscv.reg
-// CHECK-NEXT:         %[[v243:[0-9]+]] = "riscv.rem"(%[[v247]], %[[v242]]) : (!riscv.reg, !riscv.reg) -> !riscv.reg
-// CHECK-NEXT:         %[[v237:[0-9]+]] = "builtin.unrealized_conversion_cast"(%[[varg7_0]]) : (!llvm.ptr) -> !riscv.reg
-// CHECK-NEXT:         %[[v239:[0-9]+]] = "riscv.sh3add"(%[[v312]], %[[v237]]) : (!riscv.reg, !riscv.reg) -> !riscv.reg
-// CHECK-NEXT:         "riscv.sd"(%[[v239]], %[[v255]]) <{"value" = 0 : i64}> : (!riscv.reg, !riscv.reg) -> ()
-// CHECK-NEXT:         %[[v230:[0-9]+]] = "builtin.unrealized_conversion_cast"(%[[varg7_0]]) : (!llvm.ptr) -> !riscv.reg
-// CHECK-NEXT:         %[[v232:[0-9]+]] = "riscv.sh3add"(%[[v297]], %[[v230]]) : (!riscv.reg, !riscv.reg) -> !riscv.reg
-// CHECK-NEXT:         "riscv.sd"(%[[v232]], %[[v243]]) <{"value" = 0 : i64}> : (!riscv.reg, !riscv.reg) -> ()
+// CHECK-NEXT:         %[[v344:[0-9]+]] = "riscv.mul"(%[[varg27_3]], %[[varg42_0]]) : (!riscv.reg, !riscv.reg) -> !riscv.reg
+// CHECK-NEXT:         %[[v340:[0-9]+]] = "riscv.add"(%[[varg49_0]], %[[v344]]) : (!riscv.reg, !riscv.reg) -> !riscv.reg
+// CHECK-NEXT:         %[[v334:[0-9]+]] = "builtin.unrealized_conversion_cast"(%[[varg7_0]]) : (!llvm.ptr) -> !riscv.reg
+// CHECK-NEXT:         %[[v336:[0-9]+]] = "riscv.sh3add"(%[[v340]], %[[v334]]) : (!riscv.reg, !riscv.reg) -> !riscv.reg
+// CHECK-NEXT:         %[[v332:[0-9]+]] = "riscv.ld"(%[[v336]]) <{"value" = 0 : i64}> : (!riscv.reg) -> !riscv.reg
+// CHECK-NEXT:         %[[v390:[0-9]+]] = "riscv.srli"(%[[varg27_3]]) <{"value" = 63 : i64}> : (!riscv.reg) -> !riscv.reg
+// CHECK-NEXT:         %[[v147:[0-9]+]] = "riscv.add"(%[[varg27_3]], %[[v390]]) : (!riscv.reg, !riscv.reg) -> !riscv.reg
+// CHECK-NEXT:         %[[v148:[0-9]+]] = "riscv.srai"(%[[v147]]) <{"value" = 1 : i64}> : (!riscv.reg) -> !riscv.reg
+// CHECK-NEXT:         %[[v329:[0-9]+]] = "riscv.add"(%[[v148]], %[[v340]]) : (!riscv.reg, !riscv.reg) -> !riscv.reg
+// CHECK-NEXT:         %[[v323:[0-9]+]] = "builtin.unrealized_conversion_cast"(%[[varg7_0]]) : (!llvm.ptr) -> !riscv.reg
+// CHECK-NEXT:         %[[v325:[0-9]+]] = "riscv.sh3add"(%[[v329]], %[[v323]]) : (!riscv.reg, !riscv.reg) -> !riscv.reg
+// CHECK-NEXT:         %[[v321:[0-9]+]] = "riscv.ld"(%[[v325]]) <{"value" = 0 : i64}> : (!riscv.reg) -> !riscv.reg
+// CHECK-NEXT:         %[[v318:[0-9]+]] = "riscv.mul"(%[[varg49_0]], %[[v378]]) : (!riscv.reg, !riscv.reg) -> !riscv.reg
+// CHECK-NEXT:         %[[v142:[0-9]+]] = "riscv.addi"(%[[v318]]) <{"value" = 1 : i64}> : (!riscv.reg) -> !riscv.reg
+// CHECK-NEXT:         %[[v314:[0-9]+]] = "riscv.mul"(%[[varg27_1]], %[[v142]]) : (!riscv.reg, !riscv.reg) -> !riscv.reg
+// CHECK-NEXT:         %[[v308:[0-9]+]] = "builtin.unrealized_conversion_cast"(%[[varg7_3]]) : (!llvm.ptr) -> !riscv.reg
+// CHECK-NEXT:         %[[v310:[0-9]+]] = "riscv.sh3add"(%[[v314]], %[[v308]]) : (!riscv.reg, !riscv.reg) -> !riscv.reg
+// CHECK-NEXT:         %[[v306:[0-9]+]] = "riscv.ld"(%[[v310]]) <{"value" = 0 : i64}> : (!riscv.reg) -> !riscv.reg
+// CHECK-NEXT:         %[[v303:[0-9]+]] = "riscv.mul"(%[[v321]], %[[v306]]) : (!riscv.reg, !riscv.reg) -> !riscv.reg
+// CHECK-NEXT:         %[[v298:[0-9]+]] = "builtin.unrealized_conversion_cast"(%[[varg7_2]]) : (i64) -> !riscv.reg
+// CHECK-NEXT:         %[[v299:[0-9]+]] = "riscv.rem"(%[[v303]], %[[v298]]) : (!riscv.reg, !riscv.reg) -> !riscv.reg
+// CHECK-NEXT:         %[[v295:[0-9]+]] = "riscv.add"(%[[v299]], %[[v332]]) : (!riscv.reg, !riscv.reg) -> !riscv.reg
+// CHECK-NEXT:         %[[v290:[0-9]+]] = "builtin.unrealized_conversion_cast"(%[[varg7_2]]) : (i64) -> !riscv.reg
+// CHECK-NEXT:         %[[v291:[0-9]+]] = "riscv.rem"(%[[v295]], %[[v290]]) : (!riscv.reg, !riscv.reg) -> !riscv.reg
+// CHECK-NEXT:         %[[v287:[0-9]+]] = "riscv.sub"(%[[v332]], %[[v299]]) : (!riscv.reg, !riscv.reg) -> !riscv.reg
+// CHECK-NEXT:         %[[v282:[0-9]+]] = "builtin.unrealized_conversion_cast"(%[[varg7_2]]) : (i64) -> !riscv.reg
+// CHECK-NEXT:         %[[v283:[0-9]+]] = "riscv.add"(%[[v282]], %[[v287]]) : (!riscv.reg, !riscv.reg) -> !riscv.reg
+// CHECK-NEXT:         %[[v278:[0-9]+]] = "builtin.unrealized_conversion_cast"(%[[varg7_2]]) : (i64) -> !riscv.reg
+// CHECK-NEXT:         %[[v279:[0-9]+]] = "riscv.rem"(%[[v283]], %[[v278]]) : (!riscv.reg, !riscv.reg) -> !riscv.reg
+// CHECK-NEXT:         %[[v273:[0-9]+]] = "builtin.unrealized_conversion_cast"(%[[varg7_0]]) : (!llvm.ptr) -> !riscv.reg
+// CHECK-NEXT:         %[[v275:[0-9]+]] = "riscv.sh3add"(%[[v340]], %[[v273]]) : (!riscv.reg, !riscv.reg) -> !riscv.reg
+// CHECK-NEXT:         "riscv.sd"(%[[v275]], %[[v291]]) <{"value" = 0 : i64}> : (!riscv.reg, !riscv.reg) -> ()
+// CHECK-NEXT:         %[[v266:[0-9]+]] = "builtin.unrealized_conversion_cast"(%[[varg7_0]]) : (!llvm.ptr) -> !riscv.reg
+// CHECK-NEXT:         %[[v268:[0-9]+]] = "riscv.sh3add"(%[[v329]], %[[v266]]) : (!riscv.reg, !riscv.reg) -> !riscv.reg
+// CHECK-NEXT:         "riscv.sd"(%[[v268]], %[[v279]]) <{"value" = 0 : i64}> : (!riscv.reg, !riscv.reg) -> ()
 // CHECK-NEXT:         "riscv_cf.branch"() [^[[bb80:[0-9]+]]] : () -> ()
 // CHECK-NEXT:       ^[[bb80]]():
-// CHECK-NEXT:         %[[v225:[0-9]+]] = "riscv.add"(%[[v368]], %[[varg49_0]]) : (!riscv.reg, !riscv.reg) -> !riscv.reg
-// CHECK-NEXT:         "riscv_cf.branch"(%[[v225]]) [^[[bb49]]] : (!riscv.reg) -> ()
+// CHECK-NEXT:         %[[v139:[0-9]+]] = "riscv.addi"(%[[varg49_0]]) <{"value" = 1 : i64}> : (!riscv.reg) -> !riscv.reg
+// CHECK-NEXT:         "riscv_cf.branch"(%[[v139]]) [^[[bb49]]] : (!riscv.reg) -> ()
 // CHECK-NEXT:       ^[[bb54]]():
 // CHECK-NEXT:         "riscv_cf.branch"() [^[[bb84:[0-9]+]]] : () -> ()
 // CHECK-NEXT:       ^[[bb84]]():
-// CHECK-NEXT:         %[[v221:[0-9]+]] = "riscv.add"(%[[v368]], %[[varg42_0]]) : (!riscv.reg, !riscv.reg) -> !riscv.reg
-// CHECK-NEXT:         "riscv_cf.branch"(%[[v221]]) [^[[bb42]]] : (!riscv.reg) -> ()
+// CHECK-NEXT:         %[[v136:[0-9]+]] = "riscv.addi"(%[[varg42_0]]) <{"value" = 1 : i64}> : (!riscv.reg) -> !riscv.reg
+// CHECK-NEXT:         "riscv_cf.branch"(%[[v136]]) [^[[bb42]]] : (!riscv.reg) -> ()
 // CHECK-NEXT:       ^[[bb47]]():
-// CHECK-NEXT:         %[[v217:[0-9]+]] = "riscv.div"(%[[varg27_1]], %[[v370]]) : (!riscv.reg, !riscv.reg) -> !riscv.reg
-// CHECK-NEXT:         %[[v210:[0-9]+]] = "builtin.unrealized_conversion_cast"(%[[varg7_4]]) : (i64) -> !riscv.reg
-// CHECK-NEXT:         %[[v377:[0-9]+]] = "rv64.get_register"() : () -> !riscv.reg<x0>
-// CHECK-NEXT:         %[[v213:[0-9]+]] = "riscv.sltu"(%[[v377]], %[[v210]]) : (!riscv.reg<x0>, !riscv.reg) -> !riscv.reg
-// CHECK-NEXT:         %[[v214:[0-9]+]] = "builtin.unrealized_conversion_cast"(%[[v213]]) : (!riscv.reg) -> i1
-// CHECK-NEXT:         %[[v130:[0-9]+]] = "builtin.unrealized_conversion_cast"(%[[v214]]) : (i1) -> !riscv.reg
-// CHECK-NEXT:         "riscv_cf.bnez"(%[[v130]]) [^[[bb90:[0-9]+]], ^[[bb91:[0-9]+]]] <{"operandSegmentSizes" = array<i32: 1, 0, 0>}> : (!riscv.reg) -> ()
+// CHECK-NEXT:         %[[v391:[0-9]+]] = "riscv.srli"(%[[varg27_1]]) <{"value" = 63 : i64}> : (!riscv.reg) -> !riscv.reg
+// CHECK-NEXT:         %[[v132:[0-9]+]] = "riscv.add"(%[[varg27_1]], %[[v391]]) : (!riscv.reg, !riscv.reg) -> !riscv.reg
+// CHECK-NEXT:         %[[v133:[0-9]+]] = "riscv.srai"(%[[v132]]) <{"value" = 1 : i64}> : (!riscv.reg) -> !riscv.reg
+// CHECK-NEXT:         %[[v258:[0-9]+]] = "builtin.unrealized_conversion_cast"(%[[varg7_4]]) : (i64) -> !riscv.reg
+// CHECK-NEXT:         %[[v385:[0-9]+]] = "rv64.get_register"() : () -> !riscv.reg<x0>
+// CHECK-NEXT:         %[[v261:[0-9]+]] = "riscv.sltu"(%[[v385]], %[[v258]]) : (!riscv.reg<x0>, !riscv.reg) -> !riscv.reg
+// CHECK-NEXT:         %[[v262:[0-9]+]] = "builtin.unrealized_conversion_cast"(%[[v261]]) : (!riscv.reg) -> i1
+// CHECK-NEXT:         %[[v190:[0-9]+]] = "builtin.unrealized_conversion_cast"(%[[v262]]) : (i1) -> !riscv.reg
+// CHECK-NEXT:         "riscv_cf.bnez"(%[[v190]]) [^[[bb90:[0-9]+]], ^[[bb91:[0-9]+]]] <{"operandSegmentSizes" = array<i32: 1, 0, 0>}> : (!riscv.reg) -> ()
 // CHECK-NEXT:       ^[[bb90]]():
-// CHECK-NEXT:         %[[v208:[0-9]+]] = "riscv.div"(%[[varg27_3]], %[[v370]]) : (!riscv.reg, !riscv.reg) -> !riscv.reg
-// CHECK-NEXT:         "riscv_cf.branch"(%[[v208]]) [^[[bb94:[0-9]+]]] : (!riscv.reg) -> ()
+// CHECK-NEXT:         %[[v392:[0-9]+]] = "riscv.srli"(%[[varg27_3]]) <{"value" = 63 : i64}> : (!riscv.reg) -> !riscv.reg
+// CHECK-NEXT:         %[[v126:[0-9]+]] = "riscv.add"(%[[varg27_3]], %[[v392]]) : (!riscv.reg, !riscv.reg) -> !riscv.reg
+// CHECK-NEXT:         %[[v127:[0-9]+]] = "riscv.srai"(%[[v126]]) <{"value" = 1 : i64}> : (!riscv.reg) -> !riscv.reg
+// CHECK-NEXT:         "riscv_cf.branch"(%[[v127]]) [^[[bb94:[0-9]+]]] : (!riscv.reg) -> ()
 // CHECK-NEXT:       ^[[bb91]]():
-// CHECK-NEXT:         %[[v204:[0-9]+]] = "riscv.add"(%[[varg27_3]], %[[varg27_3]]) : (!riscv.reg, !riscv.reg) -> !riscv.reg
-// CHECK-NEXT:         "riscv_cf.branch"(%[[v204]]) [^[[bb94]]] : (!riscv.reg) -> ()
+// CHECK-NEXT:         %[[v256:[0-9]+]] = "riscv.add"(%[[varg27_3]], %[[varg27_3]]) : (!riscv.reg, !riscv.reg) -> !riscv.reg
+// CHECK-NEXT:         "riscv_cf.branch"(%[[v256]]) [^[[bb94]]] : (!riscv.reg) -> ()
 // CHECK-NEXT:       ^[[bb94]](%[[varg94_0:[a-zA-Z0-9_]+]] : !riscv.reg):
-// CHECK-NEXT:         %[[v197:[0-9]+]] = "builtin.unrealized_conversion_cast"(%[[varg7_4]]) : (i64) -> !riscv.reg
-// CHECK-NEXT:         %[[v378:[0-9]+]] = "rv64.get_register"() : () -> !riscv.reg<x0>
-// CHECK-NEXT:         %[[v200:[0-9]+]] = "riscv.sltu"(%[[v378]], %[[v197]]) : (!riscv.reg<x0>, !riscv.reg) -> !riscv.reg
-// CHECK-NEXT:         %[[v201:[0-9]+]] = "builtin.unrealized_conversion_cast"(%[[v200]]) : (!riscv.reg) -> i1
-// CHECK-NEXT:         %[[v161:[0-9]+]] = "builtin.unrealized_conversion_cast"(%[[v201]]) : (i1) -> !riscv.reg
-// CHECK-NEXT:         "riscv_cf.bnez"(%[[v161]]) [^[[bb99:[0-9]+]], ^[[bb100:[0-9]+]]] <{"operandSegmentSizes" = array<i32: 1, 0, 0>}> : (!riscv.reg) -> ()
+// CHECK-NEXT:         %[[v249:[0-9]+]] = "builtin.unrealized_conversion_cast"(%[[varg7_4]]) : (i64) -> !riscv.reg
+// CHECK-NEXT:         %[[v386:[0-9]+]] = "rv64.get_register"() : () -> !riscv.reg<x0>
+// CHECK-NEXT:         %[[v252:[0-9]+]] = "riscv.sltu"(%[[v386]], %[[v249]]) : (!riscv.reg<x0>, !riscv.reg) -> !riscv.reg
+// CHECK-NEXT:         %[[v253:[0-9]+]] = "builtin.unrealized_conversion_cast"(%[[v252]]) : (!riscv.reg) -> i1
+// CHECK-NEXT:         %[[v221:[0-9]+]] = "builtin.unrealized_conversion_cast"(%[[v253]]) : (i1) -> !riscv.reg
+// CHECK-NEXT:         "riscv_cf.bnez"(%[[v221]]) [^[[bb99:[0-9]+]], ^[[bb100:[0-9]+]]] <{"operandSegmentSizes" = array<i32: 1, 0, 0>}> : (!riscv.reg) -> ()
 // CHECK-NEXT:       ^[[bb99]]():
-// CHECK-NEXT:         %[[v195:[0-9]+]] = "riscv.add"(%[[varg27_0]], %[[varg27_0]]) : (!riscv.reg, !riscv.reg) -> !riscv.reg
-// CHECK-NEXT:         "riscv_cf.branch"(%[[v195]]) [^[[bb103:[0-9]+]]] : (!riscv.reg) -> ()
+// CHECK-NEXT:         %[[v247:[0-9]+]] = "riscv.add"(%[[varg27_0]], %[[varg27_0]]) : (!riscv.reg, !riscv.reg) -> !riscv.reg
+// CHECK-NEXT:         "riscv_cf.branch"(%[[v247]]) [^[[bb103:[0-9]+]]] : (!riscv.reg) -> ()
 // CHECK-NEXT:       ^[[bb100]]():
-// CHECK-NEXT:         %[[v191:[0-9]+]] = "riscv.div"(%[[varg27_0]], %[[v370]]) : (!riscv.reg, !riscv.reg) -> !riscv.reg
-// CHECK-NEXT:         "riscv_cf.branch"(%[[v191]]) [^[[bb103]]] : (!riscv.reg) -> ()
+// CHECK-NEXT:         %[[v393:[0-9]+]] = "riscv.srli"(%[[varg27_0]]) <{"value" = 63 : i64}> : (!riscv.reg) -> !riscv.reg
+// CHECK-NEXT:         %[[v120:[0-9]+]] = "riscv.add"(%[[varg27_0]], %[[v393]]) : (!riscv.reg, !riscv.reg) -> !riscv.reg
+// CHECK-NEXT:         %[[v121:[0-9]+]] = "riscv.srai"(%[[v120]]) <{"value" = 1 : i64}> : (!riscv.reg) -> !riscv.reg
+// CHECK-NEXT:         "riscv_cf.branch"(%[[v121]]) [^[[bb103]]] : (!riscv.reg) -> ()
 // CHECK-NEXT:       ^[[bb103]](%[[varg103_0:[a-zA-Z0-9_]+]] : !riscv.reg):
 // CHECK-NEXT:         "riscv_cf.branch"() [^[[bb107:[0-9]+]]] : () -> ()
 // CHECK-NEXT:       ^[[bb107]]():
-// CHECK-NEXT:         %[[v187:[0-9]+]] = "riscv.add"(%[[v368]], %[[varg27_2]]) : (!riscv.reg, !riscv.reg) -> !riscv.reg
-// CHECK-NEXT:         "riscv_cf.branch"(%[[varg103_0]], %[[v217]], %[[v187]], %[[varg94_0]]) [^[[bb27]]] : (!riscv.reg, !riscv.reg, !riscv.reg, !riscv.reg) -> ()
+// CHECK-NEXT:         %[[v115:[0-9]+]] = "riscv.addi"(%[[varg27_2]]) <{"value" = 1 : i64}> : (!riscv.reg) -> !riscv.reg
+// CHECK-NEXT:         "riscv_cf.branch"(%[[varg103_0]], %[[v133]], %[[v115]], %[[varg94_0]]) [^[[bb27]]] : (!riscv.reg, !riscv.reg, !riscv.reg, !riscv.reg) -> ()
 // CHECK-NEXT:       ^[[bb40]]():
 // CHECK-NEXT:         "llvm.return"() : () -> ()
 // CHECK-NEXT:     }) : () -> ()
